theories/lang/steps_wf.v
@@ -54,6 +54,14 @@ Lemma wf_mem_tag_mono h :
   Proper ((≤)%nat ==> impl) (wf_mem_tag h).
 Proof. move => ??? WF ??? /WF /=. lia. Qed.
 
+(** NoDup for tagged item *)
+Lemma stack_item_tagged_NoDup_singleton it:
+  stack_item_tagged_NoDup [it].
+Proof.
+  rewrite /stack_item_tagged_NoDup filter_cons filter_nil.
+  case decide => ? /=. apply NoDup_singleton. apply NoDup_nil_2.
+Qed.
+
 (** Alloc *)
 Lemma alloc_step_wf (σ σ': state) e e' h0 l bor T:
   mem_expr_step σ.(shp) e (AllocEvt l bor T) h0 e' →
@@ -79,7 +87,7 @@ Proof.
     + intros ??. rewrite init_stacks_foldr.
       intros [->|Eq]%foldr_gmap_insert_lookup; split.
       * intros si ->%elem_of_list_singleton. simpl. split; [lia|done].
-      * intros ??. set_solver.
+      * apply stack_item_tagged_NoDup_singleton.
       * move => si /(proj1 (state_wf_stack_item _ WF _ _ Eq)) /= [Lt ?].
         split; [|done]. destruct si.(tg); [simpl; lia|done..].
       * apply (state_wf_stack_item _ WF _ _ Eq).
@@ -288,7 +296,7 @@ Qed.
 Lemma for_each_lookup_case α l n f α' :
   for_each α l n false f = Some α' →
   ∀ l' stk stk', α !! l' = Some stk → α' !! l' = Some stk' →
-  stk = stk' ∨ f stk = Some stk'.
+  stk = stk' ∨ f stk = Some stk' ∧ ∃ i, (0 ≤ i < n) ∧ l' = l +ₗ i.
 Proof.
   intros EQ. destruct (for_each_lookup  _ _ _ _ _ EQ) as [EQ1 [EQ2 EQ3]].
   intros l1 stk stk' Eq Eq'.
@@ -299,7 +307,9 @@ Proof.
       rewrite /shift_loc /= Z2Nat.id; [|lia]. f_equal. lia. }
     destruct (EQ2 (Z.to_nat (l1.2 - l.2)) stk') as [stk1 [Eq1 Eq2]];
       [rewrite -(Nat2Z.id n) -Z2Nat.inj_lt; lia|by rewrite -Eql2 |].
-    rewrite -Eql2 in Eq1. simplify_eq. by right.
+    rewrite -Eql2 in Eq1. simplify_eq. right. split; [done|].
+    exists (Z.to_nat (l1.2 - l.2)). rewrite -Eql2. split; [|done].
+    rewrite Z2Nat.id; lia.
   - left. rewrite EQ3 in Eq'; [by simplify_eq|].
     intros i Lt Eq3. apply NIN. rewrite Eq3 /=. lia.
   - left. rewrite EQ3 in Eq'; [by simplify_eq|].
@@ -450,94 +460,136 @@ Proof.
   move => /for_each_access1 EQ1 WF ?? /EQ1 [? [? [? NE]]]. by eapply NE, WF.
 Qed.
 
-Lemma stack_item_no_dup_mono stk stk' :
-  stk' ⊆ stk →
-  stack_item_no_dup stk → stack_item_no_dup stk'.
-Proof. intros SUB ND it1 it2 t In1 In2. by apply ND; apply SUB. Qed.
+(* TODO: move *)
+Lemma list_subseteq_nil_sublist {A: Type} (x: list A):
+  x ⊆ [] → sublist x [].
+Proof. destruct x; set_solver. Qed.
 
-(* Lemma stack_item_no_dup_cons_1 si stk t :
-   stack_item_no_dup (si :: stk) → si.(tg) = Tagged t → ¬ si ∈ stk.
+Lemma list_subseteq_nil_inv {A: Type} (x: list A):
+  x ⊆ [] → x = [].
 Proof.
-  revert si. induction stk as [|si' stk IH]; [set_solver|].
-  intros si ND. *)
+  intros. apply : anti_symm.
+  by apply list_subseteq_nil_sublist. by apply sublist_nil_l.
+Qed.
 
-(* Lemma stack_item_no_dup_cons si stk :
-  stack_item_no_dup (si :: stk) ↔
-  (∀ t, si.(tg) = Tagged t → ¬ si ∈ stk ∧
-    ∀  si', si' ∈ stk → si'.(tg) ≠ (Tagged t)) ∧ stack_item_no_dup stk.
+Lemma NoDup_sublist {A: Type} (x y: list A) (SUB: sublist x y) :
+  NoDup y → NoDup x.
 Proof.
-  split.
-  - intros ND. split.
-    + intros t Eqsi. admit.
-    + eapply stack_item_no_dup_mono; [|exact ND]. set_solver.
-  - move => [NS ND] it1 it2 t /elem_of_cons[?|In1] /elem_of_cons[?|In2];
-      subst; [done|..].
-    + intros Eq1 Eq2. exfalso.
-      destruct (NS _ Eq1) as [? NS2]. by apply (NS2 _ In2 Eq2).
-    + intros Eq1 Eq2. exfalso.
-      destruct (NS _ Eq2) as [? NS1]. by apply (NS1 _ In1 Eq1).
-    + by apply ND. *)
+  induction SUB as [|???? IH|???? IH].
+  - done.
+  - move => /NoDup_cons [NI /IH ND]. apply NoDup_cons. split; [|done].
+    move => In1. apply NI. move : In1. by apply elem_of_list_sublist_proper.
+  - move => /NoDup_cons [NI /IH //].
+Qed.
 
-(* Lemma stack_item_no_dup_app stk1 stk2 :
-  stack_item_no_dup (stk1 ++ stk2) ↔
-  stack_item_no_dup stk1 ∧
-  (∀ t pm1 opro1 pm2 opro2,
-    mkItem pm1 (Tagged t) opro1 ∈ stk1 →
-    mkItem pm2 (Tagged t) opro2 ∈ stk2 → False) ∧
-  stack_item_no_dup stk2.
+Instance NoDup_sublist_proper {A: Type} :
+  Proper (sublist ==> flip impl) (@NoDup A).
+Proof. intros ????. by eapply NoDup_sublist. Qed.
+
+Lemma filter_sublist {A: Type} (P : A → Prop)
+  `{∀ x, Decision (P x)} (x y: list A) :
+  sublist x y → sublist (filter P x) (filter P y).
 Proof.
-  revert stk2. induction stk1 as [|si stk1 IH]; simpl; intros stk2.
-  { split; [|naive_solver].
-    intros ND. split; last split; [intros ?; set_solver|set_solver|done]. }
-  split.
-  - intros ND. split; last split.
-    + eapply stack_item_no_dup_mono; [|exact ND]. set_solver.
-    + have ND3: stack_item_no_dup (stk1 ++ stk2).
-      { eapply stack_item_no_dup_mono; [|exact ND]. set_solver. }
-      apply IH in ND3 as (ND1 & NS & ND2).
-      move => t pm1 opro1 pm2 opro2 /elem_of_cons [?|]; [|by apply NS].
-      NoDup_app
-      admit.
-    + eapply stack_item_no_dup_mono; [|exact ND]. set_solver.
-  - intros (ND1 & NS & ND2).
-    have ND3: stack_item_no_dup (stk1 ++ stk2).
-    { apply IH. split; last split; [..|done].
-      - eapply stack_item_no_dup_mono; [|exact ND1]. set_solver.
-      - intros t pm1 opro1 pm2 opro2 In1. eapply NS. right. eauto. }
-    intros it1 it2 t. rewrite 2!elem_of_cons.
-    move => [?|/elem_of_app[In1|In1]] [?|/elem_of_app[In2|In2]]; subst; [done|..].
-    + apply ND1; [by left|by right].
-    + intros Eq1 Eq2. exfalso.
-      apply (NS t si.(perm) si.(protector) it2.(perm) it2.(protector)).
-      * apply elem_of_cons. left. rewrite -Eq1. by destruct si.
-      * rewrite -Eq2. by destruct it2.
-    + apply ND1; [by right|by left].
-    + apply ND3; set_solver.
-    + apply ND3; set_solver.
-    + intros Eq1 Eq2. exfalso.
-      apply (NS t si.(perm) si.(protector) it1.(perm) it1.(protector)).
-      * apply elem_of_cons. left. rewrite -Eq2. by destruct si.
-      * rewrite -Eq1. by destruct it1.
-    + apply ND3; set_solver.
-    + by apply ND2.
-Qed. *)
+  induction 1 as [|???? IH|???? IH].
+  - done.
+  - rewrite 2!filter_cons. case decide => ? //. by constructor 2.
+  - rewrite filter_cons. case decide => ? //. by constructor 3.
+Qed.
 
-Lemma remove_check_stack_item_no_dup cids stk stk' idx:
+Lemma filter_app {A: Type} (P : A → Prop)
+  `{∀ x, Decision (P x)} (x y: list A) :
+  filter P (x ++ y) = filter P x ++ filter P y.
+Proof.
+  induction x as [|a x IH]; [done|].
+  rewrite -app_comm_cons 2!filter_cons.
+  case decide => ? //. by rewrite -app_comm_cons IH.
+Qed.
+
+(* end TODO: move *)
+
+Lemma stack_item_tagged_NoDup_cons_1 it stk :
+  stack_item_tagged_NoDup (it :: stk) → stack_item_tagged_NoDup stk.
+Proof.
+  rewrite /stack_item_tagged_NoDup filter_cons.
+  case decide => [NT|IT //]. rewrite fmap_cons. by apply NoDup_cons_12.
+Qed.
+
+Lemma stack_item_tagged_NoDup_sublist stk1 stk2:
+  sublist stk1 stk2 → stack_item_tagged_NoDup stk2 → stack_item_tagged_NoDup stk1.
+Proof.
+  intros SUB. rewrite /stack_item_tagged_NoDup.
+  by apply NoDup_sublist, fmap_sublist, filter_sublist.
+Qed.
+
+Lemma replace_check'_stack_item_tagged_NoDup cids acc stk stk':
+  replace_check' cids acc stk = Some stk' →
+  stack_item_tagged_NoDup (acc ++ stk) → stack_item_tagged_NoDup stk'.
+Proof.
+  revert acc stk'.
+  induction stk as [|it stk IH]; intros acc stk'; simpl.
+  { intros ?. simplify_eq. by rewrite app_nil_r. }
+  case decide => ?; [case check_protector; [|done]|];
+    move => /IH; [|by rewrite -app_assoc].
+  move => IH1 ND. apply IH1. clear IH1. move : ND.
+  rewrite /stack_item_tagged_NoDup 3!filter_app 2!filter_cons.
+  case decide => [IT|NT].
+  - by rewrite decide_True // 3!fmap_app 2!fmap_cons /= -assoc.
+  - by rewrite decide_False // /= filter_nil app_nil_r.
+Qed.
+
+Lemma replace_check'_stack_item_tagged_NoDup_2 cids acc stk stk' stk0:
+  replace_check' cids acc stk = Some stk' →
+  stack_item_tagged_NoDup (acc ++ stk ++ stk0) → stack_item_tagged_NoDup (stk' ++ stk0).
+Proof.
+  revert acc stk' stk0.
+  induction stk as [|it stk IH]; intros acc stk' stk0; simpl.
+  { intros ?. by simplify_eq. }
+  case decide => ?; [case check_protector; [|done]|];
+    move => /IH; [|rewrite (app_assoc acc [it] (stk ++ stk0)); naive_solver].
+  move => IH1 ND. apply IH1. clear IH1. move : ND.
+  rewrite /stack_item_tagged_NoDup 3!filter_app 2!filter_cons.
+  case decide => [IT|NT].
+  - by rewrite decide_True // 3!fmap_app 2!fmap_cons /= -assoc.
+  - by rewrite decide_False // /= filter_nil app_nil_r.
+Qed.
+
+Lemma replace_check_stack_item_tagged_NoDup cids stk stk' :
+  replace_check cids stk = Some stk' →
+  stack_item_tagged_NoDup stk → stack_item_tagged_NoDup stk'.
+Proof. intros. eapply replace_check'_stack_item_tagged_NoDup; eauto. Qed.
+
+Lemma replace_check_stack_item_tagged_NoDup_2 cids stk stk' stk0:
+  replace_check cids stk = Some stk' →
+  stack_item_tagged_NoDup (stk ++ stk0) → stack_item_tagged_NoDup (stk' ++ stk0).
+Proof. intros; eapply replace_check'_stack_item_tagged_NoDup_2; eauto. Qed.
+
+Lemma remove_check_stack_item_tagged_NoDup cids stk stk' idx:
   remove_check cids stk idx = Some stk' →
-  stack_item_no_dup stk → stack_item_no_dup stk'.
+  stack_item_tagged_NoDup stk → stack_item_tagged_NoDup stk'.
 Proof.
   revert stk' idx.
   induction stk as [|it stk IH]; intros stk' idx; simpl.
   { destruct idx; [|done]. intros ??. by simplify_eq. }
   destruct idx as [|idx]; [intros ??; by simplify_eq|].
   case check_protector eqn:Eq; [|done].
-  move => /IH IH' ND. apply IH'. eapply stack_item_no_dup_mono; [|exact ND].
-  set_solver.
+  move => /IH IH' ND. apply IH'. by eapply stack_item_tagged_NoDup_cons_1.
 Qed.
 
-Lemma access1_stack_item_no_dup stk kind bor cids n stk' :
+Lemma remove_check_stack_item_tagged_NoDup_2 cids stk stk' stk0 idx:
+  remove_check cids stk idx = Some stk' →
+  stack_item_tagged_NoDup (stk ++ stk0) → stack_item_tagged_NoDup (stk' ++ stk0).
+Proof.
+  revert stk' stk0 idx.
+  induction stk as [|it stk IH]; intros stk' stk0 idx; simpl.
+  { destruct idx; [|done]. intros ??. by simplify_eq. }
+  destruct idx as [|idx]; [intros ??; by simplify_eq|].
+  case check_protector eqn:Eq; [|done].
+  move => /IH IH' ND. apply IH'. by eapply stack_item_tagged_NoDup_cons_1.
+Qed.
+
+Lemma access1_stack_item_tagged_NoDup stk kind bor cids n stk' :
   access1 stk kind bor cids = Some (n, stk') →
-  stack_item_no_dup stk → stack_item_no_dup stk'.
+  stack_item_tagged_NoDup stk → stack_item_tagged_NoDup stk'.
 Proof.
   rewrite /access1. case find_granting as [gip|] eqn:Eq1; [|done].
   apply fmap_Some in Eq1 as [[i it] [[IN ?]%list_find_Some EQ]].
@@ -545,16 +597,14 @@ Proof.
   destruct kind.
   - case replace_check as [stk1|] eqn:Eqc ; [|done].
     simpl. intros ?. simplify_eq.
-    rewrite -{1}(take_drop n stk).
-    admit.
+    rewrite -{1}(take_drop n stk). move : Eqc.
+    by apply replace_check_stack_item_tagged_NoDup_2.
   - case find_first_write_incompatible as [?|]; [|done]. simpl.
     case remove_check as [?|] eqn:Eqc ; [|done].
     simpl. intros ?. simplify_eq.
-    rewrite -{1}(take_drop n stk).
-    intros ND. apply remove_check_stack_item_no_dup in Eqc.
-    + admit.
-    + eapply stack_item_no_dup_mono; [|exact ND]. set_solver.
-Admitted.
+    rewrite -{1}(take_drop n stk). move : Eqc.
+    apply remove_check_stack_item_tagged_NoDup_2.
+Qed.
 
 Lemma for_each_access1_stack_item α nxtc cids nxtp l n tg kind α' :
   for_each α l n false
@@ -566,11 +616,11 @@ Proof.
   split.
   - move => ? /SUB [? [IN [-> ->]]]. by apply (proj1 (WF _ _ Eq) _ IN).
   - clear SUB NN.
-    destruct (for_each_lookup_case _ _ _ _ _ ACC _ _ _ Eq Eq') as [?|Eqf].
+    destruct (for_each_lookup_case _ _ _ _ _ ACC _ _ _ Eq Eq') as [?|[Eqf ?]].
     { subst. by apply (WF _ _ Eq). }
     destruct (access1 stk kind tg cids) as [[]|] eqn:Eqf'; [|done].
     simpl in Eqf. simplify_eq.
-    eapply access1_stack_item_no_dup; eauto. by apply (WF _ _ Eq).
+    eapply access1_stack_item_tagged_NoDup; eauto. by apply (WF _ _ Eq).
 Qed.
 
 Lemma copy_step_wf σ σ' e e' h0 l bor T vl :
@@ -850,9 +900,39 @@ Proof.
   move => /for_each_grant EQ1 WF ?? /EQ1 [? [? [? NE]]]. by eapply NE, WF.
 Qed.
 
+Lemma grant_stack_item_tagged_NoDup stk bor new cids stk'
+  (NEW: match new.(tg) with
+        | Tagged t => ∀ it, it ∈ stk → it.(tg) ≠ new.(tg)
+        | _ => True
+        end) :
+  grant stk bor new cids = Some stk' →
+  stack_item_tagged_NoDup stk → stack_item_tagged_NoDup stk'.
+Proof.
+  rewrite /grant.
+  case find_granting as [[n pm]|]; [|done].
+  cbn -[item_insert_dedup]. destruct new.(perm). (* TODO: duplicated proofs *)
+  - case access1 as [[n1 stk1]|] eqn:Eq1; [|done]. cbn -[item_insert_dedup].
+    intros. simplify_eq.
+    admit.
+  - case find_first_write_incompatible as [n1|]; [|done].
+    simpl. intros. simplify_eq.
+    admit.
+  - case access1 as [[n1 stk1]|] eqn:Eq1; [|done]. cbn -[item_insert_dedup].
+    intros. simplify_eq.
+    admit.
+  - case access1 as [[n1 stk1]|] eqn:Eq1; [|done]. cbn -[item_insert_dedup].
+    intros. simplify_eq.
+    admit.
+Admitted.
+
 Lemma for_each_grant_stack_item α nxtc cids nxtp l n bor new α'
   (PR: match new.(protector) with Some c => (c < nxtc)%nat | _ => True end)
-  (TG: new.(tg) <t nxtp) :
+  (TG2: new.(tg) <t nxtp)
+  (NEW: match new.(tg) with
+        | Tagged t => ∀ (i: nat) stk, (i < n)%nat → α !! (l +ₗ i) = Some stk →
+                    ∀ it, it ∈ stk → it.(tg) ≠ new.(tg)
+        | _ => True
+        end) :
   for_each α l n false (λ stk, grant stk bor new cids) = Some α' →
   wf_stack_item α nxtp nxtc → wf_stack_item α' nxtp nxtc.
 Proof.
@@ -860,13 +940,27 @@ Proof.
   destruct (for_each_grant _ _ _ _ _ _ _ ACC _ _ Eq') as [stk [Eq [SUB ?]]].
   split.
   - eapply tagged_sublist_stack_item_included; [eauto|].
-    move => it /elem_of_cons [-> //|]. by apply (WF _ _ Eq).
-  - admit.
-Admitted.
+    move => it /elem_of_cons [-> //|] / (proj1 (WF _ _ Eq)) [Lt ?].
+    split; [|done]. move : Lt. destruct it.(tg); [lia|done].
+  - destruct (for_each_lookup_case _ _ _ _ _ ACC _ _ _ Eq Eq')
+      as [?|[Eqf [i [[Le Lt] ?]]]].
+    { subst. by apply (WF _ _ Eq). }
+    eapply grant_stack_item_tagged_NoDup; eauto.
+    + destruct new.(tg); [|done].
+      subst l'. intros it. apply (NEW (Z.to_nat i)).
+      * rewrite -(Nat2Z.id n) -Z2Nat.inj_lt; by lia.
+      * by rewrite Z2Nat.id.
+    + by apply (WF _ _ Eq).
+Qed.
 
 Lemma reborrowN_wf_stack α nxtc cids nxtp l n old new pm bar α'
   (PR: match bar with Some c => (c < nxtc)%nat | _ => True end)
-  (TG: new <t nxtp) :
+  (TG2: new <t nxtp)
+  (NEW: match new with
+        | Tagged t => ∀ (i: nat) stk, (i < n)%nat → α !! (l +ₗ i) = Some stk →
+                    ∀ it, it ∈ stk → it.(tg) ≠ new
+        | _ => True
+        end) :
   reborrowN α cids l n old new pm bar = Some α' →
   wf_stack_item α nxtp nxtc ∧ wf_non_empty α →
   dom (gset loc) α ≡ dom (gset loc) α' ∧
@@ -898,7 +992,7 @@ Proof.
 Qed.
 
 Lemma visit_freeze_sensitive'_wf_stack h l (f: stacks → _ → _ → _ → _)
-  α α' last cur T lc' nxtp nxtc :
+  α α' last cur T lc' nxtp nxtc:
   let Hα α1 α2 :=
     (wf_stack_item α1 nxtp nxtc ∧ wf_non_empty α1 →
       dom (gset loc) α1 ≡ dom (gset loc) α2 ∧
@@ -906,9 +1000,7 @@ Lemma visit_freeze_sensitive'_wf_stack h l (f: stacks → _ → _ → _ → _)
   let HF f α1 α2 := (∀ l n b, f α1 l n b = Some α2 → Hα α1 α2) in
   (∀ α1 α2, HF f α1 α2) →
   visit_freeze_sensitive' h l f α last cur T = Some (α', lc') →
-  wf_stack_item α nxtp nxtc ∧ wf_non_empty α →
-  dom (gset loc) α ≡ dom (gset loc) α' ∧
-  wf_stack_item α' nxtp nxtc ∧ wf_non_empty α'.
+  Hα α α'.
 Proof.
   intros Hα HF.
   apply (visit_freeze_sensitive'_elim
@@ -966,8 +1058,13 @@ Proof.
 Qed.
 
 Lemma reborrow_wf_stack h α nxtc cids nxtp l old T kind new bar α'
-  (INCL: new <t nxtp)
-  (BAR : match bar with Some c => (c < nxtc)%nat | _ => True end) :
+  (TG2: new <t nxtp)
+  (BAR : match bar with Some c => (c < nxtc)%nat | _ => True end)
+  (NEW: match new with
+        | Tagged t => ∀ (i: nat) stk, (i < tsize T)%nat → α !! (l +ₗ i) = Some stk →
+                    ∀ it, it ∈ stk → it.(tg) ≠ new
+        | _ => True
+        end) :
   reborrow h α cids l old T kind new bar = Some α' →
   wf_stack_item α nxtp nxtc ∧ wf_non_empty α →
   dom (gset loc) α ≡ dom (gset loc) α' ∧
@@ -976,7 +1073,8 @@ Proof.
   rewrite /reborrow. destruct kind as [[]| |].
   - by eapply reborrowN_wf_stack; eauto.
   - by eapply reborrowN_wf_stack; eauto.
-  - apply visit_freeze_sensitive_wf_stack.
+  - SearchAbout visit_freeze_sensitive.
+    apply visit_freeze_sensitive_wf_stack.
     intros ???????. by eapply reborrowN_wf_stack.
   - destruct mutable.
     + by eapply reborrowN_wf_stack; eauto.
